theories/partial/nonempty.v
@@ -1,0 +1,702 @@
+Require Import Coq.Logic.ProofIrrelevance.
+(* Instead of using SProp, for now I'll just use the proof irrelevance axiom.
+   I'll see if this causes any issues; probably not. *)
+Require Import FunctionalExtensionality.
+Require Import Coq.Logic.PropExtensionality.
+
+(*
+My idea is to have the monad of nonempty sets. Maybe that corresponds to choice, and
+maybe it still gets classical stuff?
+ *)
+
+Polymorphic Definition sort'@{s | u |} (T : Type@{s|u}):= Type@{s|u}.
+(*Polymorphic Definition sort@{s ; u} := Type@{s;u}.*)
+(* This second syntax is the current version of rocq *)
+Check (sort' nat).
+Check (sort' True).
+
+Polymorphic Inductive Test@{s | u|} : Type@{s | u}.
+Check Test@{Type | Type}.
+Check Test@{Prop | Type}.
+
+Polymorphic Definition test2@{s|u|} : Type@{s|u} := Test@{s|u}.
+Check test2@{Type|Type}.
+Check test2@{Prop|Type}.
+
+Polymorphic Definition test3@{s|u|} := Test@{s|u}.
+Check test3@{Type|Type}.
+Check test3@{Prop|Type}.
+Check exist.
+Definition PClassical (P : Prop) : Prop := not (not P).
+
+Definition Preturn {A : Prop} (x : A) : PClassical A.
+Proof.
+  intro na.
+  apply na.
+  apply x.
+Qed.
+
+Theorem Pbind {A B : Prop} (pa : PClassical A) (f : A -> PClassical B) : PClassical B.
+  Proof.
+  unfold PClassical in *.
+  intros nb.
+  apply pa.
+  intro a.
+  apply f.
+  - apply a.
+  - apply nb.
+Qed.
+
+Theorem Plem (P : Prop) : PClassical (P \/ ~P).
+Proof.
+  intros n.
+  apply n.
+  apply or_intror.
+  intros p.
+  apply n.
+  apply or_introl.
+  apply p.
+Qed.
+
+Definition Classical (A : Type) : Type :=
+  {S : A -> Prop | not (forall x, not (S x))}.
+Check Classical.
+Check (Classical nat).
+Check (Classical True).
+(* TODO: Is that the best way to express non-emptyness with a double negation? *)
+
+Definition Creturn {A : Type} (x : A) : Classical A.
+  refine (exist _ (fun y => y = x) _).
+  intros.
+  intros p.
+  specialize (p x).
+  contradiction.
+Defined.
+
+Theorem classicalEq :
+  forall A S1 S2 p1 p2,
+    S1 = S2 -> @eq (Classical A) (exist _ S1 p1) (exist _ S2 p2).
+Proof.
+  intros.
+  subst S1.
+  assert (p1 = p2).
+  apply proof_irrelevance.
+  subst p1.
+  reflexivity.
+Qed.
+
+Theorem classicalEq2:
+  forall A (x y : Classical A), proj1_sig x = proj1_sig y -> x = y.
+Proof.
+  intros.
+  destruct x.
+  destruct y.
+  simpl in H.
+  apply classicalEq.
+  assumption.
+Qed.
+
+Theorem CreturnInj : forall A (x y : A), Creturn x = Creturn y -> x = y.
+Proof.
+  intros.
+  pose (@f_equal _ _ (@proj1_sig _ _) _ _ H) as fact.
+  simpl in fact.
+  assert ((fun y => y = x) x).
+  reflexivity.
+  rewrite fact in H0.
+  assumption.
+Qed.
+
+Definition Cbind {A B : Type} (pa : Classical A) (f : A -> Classical B) : Classical B.
+  refine (exist _ (fun b => exists a, proj1_sig pa a /\ proj1_sig (f a) b) _).
+  destruct pa as [Sa nonempty].
+  simpl.
+  intros p.
+  apply nonempty.
+  intros a Sax.
+  remember (f a) as fa.
+  destruct fa as [SB nonemptyB].
+  apply nonemptyB.
+  intros b SBb.
+  specialize (p b).
+  apply p.
+  exists a.
+  split.
+  + apply Sax.
+  + rewrite <- Heqfa.
+    simpl.
+    apply SBb.
+Defined.
+
+Theorem bindDef : forall A B (a : A) (f : A -> Classical B),
+    Cbind (Creturn a) f = f a.
+Proof.
+  intros.
+  apply classicalEq2.
+  apply functional_extensionality.
+  intros.
+  apply propositional_extensionality.
+  split.
+  - intros.
+    simpl in H.
+    destruct H.
+    destruct H.
+    subst x0.
+    assumption.
+  - intros.
+    simpl.
+    exists a.
+    split.
+    reflexivity.
+    assumption.
+Qed.
+
+Definition Cmap {A B : Type} (f : A -> B) (c : Classical A) : Classical B
+  := Cbind c (fun a => Creturn (f a)).
+Theorem CmapDef : forall A B f a, @Cmap A B f (Creturn a) = Creturn (f a).
+Proof.
+  unfold Cmap.
+  intros.
+  rewrite bindDef.
+  reflexivity.
+Qed.
+
+(*
+TODO: Would it be better to just use normal bind + return, and then have
+a function (Classical Prop -> Prop)?
+*)
+Definition propBind {T : Type} (P : T -> Prop) (pa : Classical T) : Prop :=
+  Creturn True = (Cbind pa (fun a => Creturn (P a))).
+
+Theorem propBindDef {T : Type} (t : T) (P : T -> Prop) :
+  propBind P (Creturn t) = P t.
+Proof.
+  unfold propBind.
+  rewrite bindDef.
+  apply propositional_extensionality.
+  split.
+  - intros.
+    apply CreturnInj in H.
+    rewrite <- H.
+    apply I.
+  - intros.
+    apply (f_equal Creturn).
+    apply propositional_extensionality.
+    split; auto.
+Qed.
+
+
+Theorem doesClassicalImplyNormal (P : Prop) : Classical P -> P.
+Proof.
+  intros [S unique].
+  (* No *)
+Abort.
+
+Theorem sortOfThough (P : Prop) : Classical P -> ~~P.
+Proof.
+  intros.
+  intros np.
+  destruct X as [S nonempty].
+  apply nonempty.
+  intros x Sx.
+  apply np.
+  apply x.
+Qed.
+
+
+Theorem lem (P : Prop) : Classical (P \/ not P).
+Proof.
+  refine (exist _ (fun pornotp => True) _).
+  intros nn.
+  assert ((~True) = False). {
+    apply propositional_extensionality.
+    split; auto.
+  }
+  rewrite H in nn.
+  apply nn.
+  + apply or_intror.
+    intros p.
+    apply nn.
+    apply or_introl.
+    apply p.
+Defined.
+
+Theorem lem2 (P : Prop) : Classical (P + not P).
+Proof.
+  refine (exist _ (fun pornotp => True) _).
+  intros nn.
+  assert ((~True) = False). {
+    apply propositional_extensionality.
+    split; auto.
+  }
+  rewrite H in nn.
+  apply nn.
+  + apply inr.
+    intros p.
+    apply nn.
+    apply inl.
+    apply p.
+Defined.
+
+Definition choose (T : Type) (P : T -> Prop) (H : exists t, P t): Classical T.
+  refine (exist _ P _).
+  intros p.
+  destruct H as [t Pt].
+  specialize (p t).
+  contradiction.
+Defined.
+
+Theorem choice_spec' (T : Type) (P : T -> Prop) (H : exists t, P t)
+  : Cbind (choose T P H) (fun t => Creturn (P t)) = Creturn True.
+Proof.
+  apply classicalEq2.
+  simpl.
+  extensionality X.
+  apply propositional_extensionality.
+  split.
+  - intros.
+    destruct H0.
+    destruct H0.
+    subst.
+    apply propositional_extensionality; split; auto.
+  - intros.
+    subst.
+    destruct H.
+    exists x.
+    split; auto.
+    apply propositional_extensionality; split; auto.
+Qed.
+
+Theorem choice_spec (T : Type) (P : T -> Prop) (H : exists t, P t)
+  : propBind P (choose T P H).
+  apply classicalEq2.
+  simpl.
+  extensionality X.
+  apply propositional_extensionality.
+  split.
+
+  - intros.
+    subst.
+    destruct H.
+    exists x.
+    split; auto.
+    apply propositional_extensionality; split; auto.
+  - intros.
+    destruct H0.
+    destruct H0.
+    subst.
+    apply propositional_extensionality; split; auto.
+Qed.
+    
+Theorem ind {T : Type} : forall (P : Classical T -> Prop),
+    (forall (a : T), P (Creturn a)) -> forall (q : Classical T), (P q).
+Proof.
+  intros.
+  destruct q.
+Abort.
+
+(*
+Definition Pif {A : Type} (P : Prop) (a1 a2 : Classical A) : Classical A.
+  refine (exist _ (fun a => (P /\ proj1_sig a1 a) \/ ((not P) /\ proj1_sig a2 a)) _).
+ *)
+
+(*
+Theorem PifDef1 : forall (A : Type) P (a1 a2 : A), P -> Pif P a1 a2 = Creturn a1.
+Proof.
+  intros.
+  apply classicalEq.
+  apply functional_extensionality.
+  intros.
+  apply propositional_extensionality.
+  split.
+  - intros.
+    destruct H0.
+    destruct H0.
+    assumption.
+    destruct H0.
+    contradiction.
+  - intros.
+    subst.
+    apply or_introl.
+    split.
+    assumption.
+    reflexivity.
+Qed.
+
+Theorem PifDef2 : forall (A : Type) P (a1 a2 : A), not P -> Pif P a1 a2 = Creturn a2.
+Proof.
+  intros.
+  apply classicalEq.
+  apply functional_extensionality.
+  intros.
+  apply propositional_extensionality.
+  split.
+  - intros.
+    destruct H0.
+    + destruct H0.
+      contradiction.
+    + destruct H0.
+      assumption.
+  - intros.
+    subst.
+    apply or_intror.
+    split.
+    assumption.
+    reflexivity.
+Qed.
+*)
+(* We do need partiality for general recursion. Will this work? *)
+Definition Partial (T : Type) : Type := Classical (option T).
+
+(* better name? *)
+Definition seqOption (A B : Type) (f : A -> Partial B) : Partial (A -> Classical B).
+  refine (exist _ (fun g =>
+                     ((exists a, f a = Creturn None) /\ g = None)
+                     \/
+                       (exists g', g = Some g' /\ forall a, f a = Cmap Some (g' a))) _).
+Abort.
+(*Maybe a better design would be to put a double negation all the way around the outside of the prop part
+of classical? *)
+
+
+(*
+The question is: can I do general recursion somehow?
+ *)
+
+(* Unfortunately, sort polymorphism isn't good enough to make Classical P be able 
+ to be in Prop, so I have to make a whole separate definition.
+ This definition can be simpler (but it doesn't have to be, it could be identitcal to Classical) *)
+
+
+(*
+I think that my definition of choose needs to actually have the monad around
+the inputs as well as the output, so I can use it correctly.
+ *)
+Definition choose2 (T : Type) (P : T -> Prop) (H : PClassical (exists t, P t)): Classical T.
+  refine (exist _ P _).
+  intros p.
+  apply H.
+  intros x.
+  destruct x.
+  specialize (p x).
+  contradiction.
+Defined.
+
+Theorem choice_spec2 (T : Type) (P : T -> Prop) (H : exists t, P t)
+  : Cbind (choose T P H) (fun t => Creturn (P t)) = Creturn True.
+Proof.
+  apply classicalEq2.
+  simpl.
+  extensionality X.
+  apply propositional_extensionality.
+  split.
+  - intros.
+    destruct H0.
+    destruct H0.
+    subst.
+    apply propositional_extensionality; split; auto.
+  - intros.
+    subst.
+    destruct H.
+    exists x.
+    split; auto.
+    apply propositional_extensionality; split; auto.
+Qed.
+
+Section existT_inj2_uip.
+  Variables (A : Type) (P : A -> Type).
+
+  Implicit Type (x : A).
+  Print sigT.
+
+  Theorem exist_inj2_helper x (px : P x) (y : sigT P) :
+      @existT _ _ x px = y
+    -> exists e : x = projT1 y, eq_rect x P px _ e = projT2 y.
+  Proof using Type. intros []; exists eq_refl; auto. Qed.
+
+  Fact exists_inj2 x y (px : P x) (py : P y) :
+      existT _ x px = existT _ y py
+    -> exists e : x = y, eq_rect x P px _ e = py.
+  Proof using Type. intros (e & ?)%exist_inj2_helper. exists e; subst; simpl; auto. Qed.
+
+  Fact exist_inj2_uip :
+    forall x (p1 p2 : P x), existT _ x p1 = existT _ x p2 -> p1 = p2.
+  Proof using Type.
+    intros x p1 p2 (e & He)%exists_inj2.
+    rewrite (UIP _ _ _ e eq_refl) in He.
+    assumption.
+  Qed.
+End existT_inj2_uip.
+
+(* Using choice, returns the element of T satisfying P if it exists, otherwise None *)
+Definition chooseOption (T : Type) (P : T -> Prop) : Classical (option T).
+  Check choose.
+  refine (choose2 (option T)
+                 (fun ot => match ot with
+                            | Some t => P t
+                            | None => ~exists t, P t
+                            end) _).
+  apply (Pbind (Plem (exists t, P t))).
+  intros doesOrDoesNot.
+  destruct doesOrDoesNot.
+  - destruct H.
+    apply Preturn.
+    exists (Some x).
+    assumption.
+  - apply Preturn.
+    exists None.
+    assumption.
+Defined.
+
+Check @choose.
+
+Theorem choiceInd : forall (T : Type) (P Q : T -> Prop) x,
+    (forall t, P t -> Q t) -> Cbind (@choose2 T P x) (fun t => Creturn (Q t)) = Creturn True.
+Proof.
+  intros.
+  apply classicalEq2.
+  simpl.
+  (*the exists comes from Cbind. It needs to have a double negation on it.*)
+  extensionality X.
+  apply propositional_extensionality.
+  split.
+  - intros.
+    destruct H0.
+    destruct H0.
+    subst.
+    apply propositional_extensionality; split; auto.
+  - intros.
+    subst.
+    destruct H.
+    exists x.
+    split; auto.
+    apply propositional_extensionality; split; auto.
+Qed.
+
+Theorem chooseOptionSpec1 : forall T P t,
+    chooseOption T P = Creturn (Some t) -> P t.
+Proof.
+  intros T P t.
+  unfold chooseOption.
+  apply choiceInd.
+  intros.
+  destruct t0.
+  - inversion H0.
+    subst.
+    assumption.
+  - inversion H0.
+ Qed.  
+
+Theorem chooseOptionSpec2 : forall T P,
+    chooseOption T P = None -> ~exists t, P t.
+Proof.
+  intros T P.
+  unfold chooseOption.
+  apply choiceInd.
+  intros.
+  destruct t.
+  - inversion H0.
+  - assumption.
+ Qed.
+
+Inductive Prog (A B : Type) : Type :=
+| Ret : option B -> Prog A B
+| Rec : forall (I : Type) (args : I -> A), ((I -> B) -> Prog A B) -> Prog A B
+.
+
+Inductive runProgR {A B : Type} (def : A -> Prog A B) : Prog A B -> B -> Prop :=
+| retR : forall b, runProgR def (Ret _ _ (Some b)) b
+| recR : forall I
+                (args : I -> A)
+                (recVals : I -> B)
+                (res : B)
+                (rest : (I -> B) -> Prog A B),
+    (* if for all inputs a satisfying P, recVals describes the recursive calls *)
+    (forall (i : I), runProgR def (def (args i)) (recVals i))
+    (* and given the results of those recursive calls, the program outputs res *)
+    -> runProgR def (rest recVals) res
+    (* then overall res *)
+    -> runProgR def (Rec _ _ I args rest) res
+.
+
+Theorem runProgFunction {A B : Type} {def : A -> Prog A B} {p : Prog A B} {b1 b2 : B}
+  (rp1 : runProgR def p b1) (rp2 : runProgR def p b2) : b1 = b2.
+Proof.
+  intros.
+  generalize rp2.
+  generalize b2.
+  clear rp2.
+  clear b2.
+  induction rp1.
+  - intros.
+    inversion rp2.
+    reflexivity.
+  - intros.
+    inversion rp2.
+    apply exist_inj2_uip in H2.
+    subst.
+    apply IHrp1.
+    assert (rest1 = rest). {
+      apply exist_inj2_uip in H4.
+      assumption.
+    }
+    subst.
+    assert (recVals = recVals0). {
+      extensionality i.
+      specialize (H i).
+      specialize (H5 i).
+      apply H0.
+      apply H5.
+    }
+    subst.
+    assumption.
+Qed.
+
+Definition runProgImpl {A B : Type} (def : A -> Prog A B) (p : Prog A B) : option B.
+  refine (chooseOption B (fun b => runProgR def p b)).
+Defined.
+
+Definition runProg {A B : Type} (def : A -> Prog A B) (a : A) : option B :=
+  (runProgImpl def (def a)).
+
+Theorem runProgDefinitionRet {A B : Type} (def : A -> Prog A B) (b : option B)
+  : runProgImpl def (Ret _ _ b) = b.
+  unfold runProgImpl, chooseOption.
+  apply choiceInd.
+  intros.
+  destruct t.
+  - inversion H.
+    subst.
+    reflexivity.
+  - destruct b.
+    + exfalso.
+      apply H.
+      exists b.
+      constructor.
+    + reflexivity.
+Qed.
+     
+Theorem runProgDefinitionRec2 {A B : Type} {def : A -> Prog A B}
+        {I : Type}
+        {args : I -> A}
+        {rest : (I -> B) -> Prog A B}
+        {recVals : I -> B}
+        (recValsCorrect : forall (i : I), runProg def (args i) = Some (recVals i))
+  : runProgImpl def (Rec _ _ I args rest) = runProgImpl def (rest recVals).
+ Proof.
+   unfold runProg, runProgImpl, chooseOption in *.
+   repeat apply choiceInd.
+   intros.
+   assert (forall (i :  I), runProgR def (def (args i)) (recVals i)). {
+     intros.
+     specialize (recValsCorrect i).
+     symmetry in recValsCorrect.
+     Check choiceIndHyp.
+     apply choiceIndHyp in recValsCorrect.
+     assumption.
+   }
+   clear recValsCorrect.
+   (*H1 could have just been the input to runProgDefinitionRec2*)
+   destruct t0.
+   - inversion H0; clear H0.
+     apply exist_inj2_uip in H3, H5.
+     subst.
+     assert (recVals = recVals0). {
+       extensionality i.
+       exact (runProgFunction (H1 i) (H6 i)).
+     }
+     subst.
+     destruct t.
+     + rewrite (runProgFunction H7 H).
+       reflexivity.
+     + exfalso.
+       apply H.
+       exists b.
+       apply H7.
+   - destruct t.
+     + exfalso.
+       apply H0.
+       exists b.
+       econstructor.
+       * apply H1.
+       * assumption.
+     + reflexivity.
+ Qed.
+ 
+Theorem runProgDefinitionRec {A B : Type} {def : A -> Prog A B}
+        {I : Type}
+        {args : I -> A}
+        {rest : (I -> B) -> Prog A B}
+  : runProgImpl def (Rec _ _ I args rest) =
+      bind ((collectOption (fun i => runProg def (args i))) : option (I -> B))
+           (fun f => runProgImpl def (rest f)).
+Proof.
+  repeat unfold runProgImpl, runProg, collectOption, chooseOption.
+  repeat apply choiceInd.
+  intros.
+  destruct t.
+  -
+    assert (forall i, runProgR def (def (args i)) (b i)). {
+      intros.
+      specialize (H i).
+      apply choiceIndHyp in H.
+      assumption.
+    }
+    clear H.
+    simpl.
+    apply choiceInd.
+    intros.
+    destruct t0.
+    inversion H0; clear H0; subst.
+    + apply exist_inj2_uip in H3, H5.
+      subst.
+      assert (b = recVals). {
+        extensionality i.
+        exact (runProgFunction (H1 i) (H6 i)).
+      }
+      subst.
+      destruct t.
+      * rewrite (runProgFunction H H7).
+        reflexivity.
+      * exfalso.
+        apply H.
+        exists b0.
+        assumption.
+    + destruct t.
+      * exfalso.
+        apply H0.
+        exists b0.
+        econstructor.
+        apply H1.
+        apply H.
+      * reflexivity.
+  - simpl.
+    destruct t0.
+    + exfalso.
+      inversion H0.
+      apply H.
+      apply exist_inj2_uip in H2, H4.
+      subst.
+      exists recVals.
+      intros.
+      apply choiceInd.
+      intros.
+      destruct t.
+      * specialize (H5 a).
+        rewrite (runProgFunction H5 H1).
+        reflexivity.
+      * exfalso.
+        apply H.
+        exists recVals.
+        intros.
+        apply choiceInd.
+        intros.
+        destruct t.
+        -- rewrite (runProgFunction (H5 a0) H2).
+           reflexivity.
+        -- exfalso.
+           apply H1.
+           exists (recVals a).
+           apply H5.
+    + reflexivity.
+Qed.    
